proof/iu_system/uni/algo_worklist/def_extra.v
@@ -89,58 +89,58 @@ Inductive a_update_bound
 
 (* defns Jaworklist_reduction *)
 Inductive a_wl_red : aworklist -> Prop :=    (* defn a_wl_red *)
- | a_wlred__empty : a_wl_red aworklist_empty
- | a_wlred__gc_var : forall (Γ:aworklist) (x:expvar) (A:typ),
+ | d_wl_del__empty : a_wl_red aworklist_empty
+ | d_wl_del__gc_var : forall (Γ:aworklist) (x:expvar) (A:typ),
      a_wl_red Γ ->
      a_wl_red (aworklist_consvar Γ x (abind_typ A))
- | a_wlred__gc_tvar : forall (Γ:aworklist) (X:typvar),
+ | d_wl_del__gc_tvar : forall (Γ:aworklist) (X:typvar),
      a_wl_red Γ ->
      a_wl_red (aworklist_constvar Γ X abind_tvar_empty)
- | a_wlred__gc_stvar : forall (Γ:aworklist) (X:typvar),
+ | d_wl_del__gc_stvar : forall (Γ:aworklist) (X:typvar),
      a_wl_red Γ ->
      a_wl_red (aworklist_constvar Γ X abind_stvar_empty)
- | a_wlred__gc_etvar : forall (Γ:aworklist) (X:typvar) (A B:typ),
+ | d_wl_del__gc_etvar : forall (Γ:aworklist) (X:typvar) (A B:typ),
      a_wl_red (aworklist_conswork Γ (work_sub A B)) ->
      a_wl_red (aworklist_constvar Γ X (abind_bound A B))
- | a_wlred__sub_top : forall (Γ:aworklist) (B1:typ),
+ | d_wl_del__sub_top : forall (Γ:aworklist) (B1:typ),
      a_wl_red Γ ->
      a_wl_red (aworklist_conswork Γ (work_sub B1 typ_top))
- | a_wlred__sub_bot : forall (Γ:aworklist) (A:typ),
+ | d_wl_del__sub_bot : forall (Γ:aworklist) (A:typ),
      a_wl_red Γ ->
      a_wl_red (aworklist_conswork Γ (work_sub typ_bot A))
- | a_wlred__sub_unit : forall (Γ:aworklist),
+ | d_wl_del__sub_unit : forall (Γ:aworklist),
      a_wl_red Γ ->
      a_wl_red (aworklist_conswork Γ (work_sub typ_unit typ_unit))
- | a_wlred__sub_tvar : forall (Γ:aworklist) (X:typvar),
+ | d_wl_del__sub_tvar : forall (Γ:aworklist) (X:typvar),
      a_wl_red Γ ->
      a_wl_red (aworklist_conswork Γ (work_sub (typ_var_f X) (typ_var_f X)))
- | a_wlred__subarrow : forall (Γ:aworklist) (B1 B2 A1 A2:typ),
+ | d_wl_del__subarrow : forall (Γ:aworklist) (B1 B2 A1 A2:typ),
      a_wl_red (aworklist_conswork (aworklist_conswork Γ (work_sub A1 B1)) (work_sub B2 A2)) ->
      a_wl_red (aworklist_conswork Γ (work_sub (typ_arrow B1 B2) (typ_arrow A1 A2)))
- | a_wlred__sub_alll : forall (L:vars) (Γ:aworklist) (B1 A1:typ),
+ | d_wl_del__sub_alll : forall (L:vars) (Γ:aworklist) (B1 A1:typ),
      neq_all A1 ->
      neq_intersection A1 ->
      neq_union A1 ->
       ( forall X , X \notin  L  -> a_wl_red (aworklist_conswork (aworklist_constvar Γ X (abind_bound typ_bot typ_top)) (work_sub  ( open_typ_wrt_typ B1 (typ_var_f X) )  A1)) )  ->
      a_wl_red (aworklist_conswork Γ (work_sub (typ_all B1) A1))
- | a_wlred__sub_all : forall (L:vars) (Γ:aworklist) (B1 A1:typ),
+ | d_wl_del__sub_all : forall (L:vars) (Γ:aworklist) (B1 A1:typ),
       ( forall X , X \notin  L  -> a_wl_red (aworklist_conswork (aworklist_constvar Γ X abind_stvar_empty) (work_sub  ( open_typ_wrt_typ B1 (typ_var_f X) )   ( open_typ_wrt_typ A1 (typ_var_f X) ) )) )  ->
      a_wl_red (aworklist_conswork Γ (work_sub (typ_all B1) (typ_all A1)))
- | a_wlred__sub_arrow1 : forall (L:vars) (Γ:aworklist) (X:typvar) (A1 A2 B1 B2:typ) (X1 X2:typvar),
+ | d_wl_del__sub_arrow1 : forall (L:vars) (Γ:aworklist) (X:typvar) (A1 A2 B1 B2:typ) (X1 X2:typvar),
       binds ( X )  ( (abind_bound B1 B2) ) (  ( awl_to_aenv  Γ  )  )  ->
       ( a_smono_typ   ( awl_to_aenv  Γ  )     ( (typ_arrow A1 A2) )   -> False )  ->
       (forall X1 X2 Γ2 Γ3, X1 `notin` L -> X2 `notin` (L `union` singleton X1) ->  
         (a_update_bound  (aworklist_constvar (aworklist_constvar Γ X1 (abind_bound typ_bot typ_top)) X2 (abind_bound typ_bot typ_top))   nil   X   (typ_arrow (typ_var_f X1) (typ_var_f X2))  a_mode_ub__upper  Γ2   Γ3 ) /\ 
         (a_wl_red (aworklist_conswork  (   ( awl_app  Γ3   Γ2  )   )  (work_sub (typ_arrow (typ_var_f X1) (typ_var_f X2)) (typ_arrow A1 A2)))) ) ->
      a_wl_red (aworklist_conswork Γ (work_sub (typ_var_f X) (typ_arrow A1 A2)))
- | a_wlred__sub_arrow2 : forall (L:vars) (Γ:aworklist) (A1 A2:typ) (X:typvar) (B1 B2:typ) (X1 X2:typvar),
+ | d_wl_del__sub_arrow2 : forall (L:vars) (Γ:aworklist) (A1 A2:typ) (X:typvar) (B1 B2:typ) (X1 X2:typvar),
       binds ( X )  ( (abind_bound B1 B2) ) (  ( awl_to_aenv  Γ  )  )  ->
       ( a_smono_typ   ( awl_to_aenv  Γ  )     ( (typ_arrow A1 A2) )   -> False )  ->
       (  forall X1 X2 Γ2 Γ3, X1 `notin` L -> X2 `notin` (L `union` singleton X1) -> 
              (a_update_bound  (aworklist_constvar (aworklist_constvar Γ X1 (abind_bound typ_bot typ_top)) X2 (abind_bound typ_bot typ_top))   nil   X   (typ_arrow (typ_var_f X1) (typ_var_f X2))  a_mode_ub__lower  Γ2   Γ3 )  /\
             a_wl_red (aworklist_conswork  (   ( awl_app  Γ3   Γ2  )   )  (work_sub (typ_arrow A1 A2) (typ_arrow (typ_var_f X1) (typ_var_f X2)))) )->
      a_wl_red (aworklist_conswork Γ (work_sub (typ_arrow A1 A2) (typ_var_f X)))
- | a_wlred__sub_etvar1 : forall (L:vars) (Γ:aworklist) (Y X:typvar) (B1 B2 B3 B4:typ),
+ | d_wl_del__sub_etvar1 : forall (L:vars) (Γ:aworklist) (Y X:typvar) (B1 B2 B3 B4:typ),
       binds ( X )  ( (abind_bound B1 B2) ) (  ( awl_to_aenv  Γ  )  )  ->
       binds ( Y )  ( (abind_bound B3 B4) ) (  ( awl_to_aenv  Γ  )  )  ->     a_evs_in_wl Γ X Y ->
       a_evs_in_wl Γ X Y ->
@@ -148,7 +148,7 @@ Inductive a_wl_red : aworklist -> Prop :=    (* defn a_wl_red *)
             (a_update_bound  Γ   nil   X   (typ_var_f Y)  a_mode_ub__lower  Γ2   Γ3 )  /\
             a_wl_red  (   ( awl_app  Γ3   Γ2  )   ) ) ->
      a_wl_red (aworklist_conswork Γ (work_sub (typ_var_f Y) (typ_var_f X)))
- | a_wlred__sub_etvar2 : forall (L:vars) (Γ:aworklist) (X Y:typvar) (B1 B2 B3 B4:typ),
+ | d_wl_del__sub_etvar2 : forall (L:vars) (Γ:aworklist) (X Y:typvar) (B1 B2 B3 B4:typ),
       binds ( X )  ( (abind_bound B1 B2) ) (  ( awl_to_aenv  Γ  )  )  ->
       binds ( Y )  ( (abind_bound B3 B4) ) (  ( awl_to_aenv  Γ  )  )  ->
       a_evs_in_wl Γ X Y ->
@@ -156,137 +156,137 @@ Inductive a_wl_red : aworklist -> Prop :=    (* defn a_wl_red *)
             (a_update_bound  Γ   nil   X   (typ_var_f Y)  a_mode_ub__upper  Γ2   Γ3 )  /\
             a_wl_red  (   ( awl_app  Γ3   Γ2  )   ) ) ->
      a_wl_red (aworklist_conswork Γ (work_sub (typ_var_f X) (typ_var_f Y)))
- | a_wlred__sub_etvarmono1 : forall (L:vars) (Γ:aworklist) (A1:typ) (X:typvar) (B1 B2:typ),
+ | d_wl_del__sub_etvarmono1 : forall (L:vars) (Γ:aworklist) (A1:typ) (X:typvar) (B1 B2:typ),
       binds ( X )  ( (abind_bound B1 B2) ) (  ( awl_to_aenv  Γ  )  )  ->
      a_smono_typ  ( awl_to_aenv  Γ  )  A1 ->
      (  forall X1 X2 Γ2 Γ3, X1 `notin` L -> X2 `notin` (L `union` singleton X1) -> 
             (a_update_bound  Γ   nil   X   A1  a_mode_ub__lower  Γ2   Γ3 )  /\
             a_wl_red  (   ( awl_app  Γ3   Γ2  )   ) ) ->
      a_wl_red (aworklist_conswork Γ (work_sub A1 (typ_var_f X)))
- | a_wlred__sub_etvarmono2 : forall (L:vars) (Γ:aworklist) (X:typvar) (B1 A1 A2:typ),
+ | d_wl_del__sub_etvarmono2 : forall (L:vars) (Γ:aworklist) (X:typvar) (B1 A1 A2:typ),
       binds ( X )  ( (abind_bound A1 A2) ) (  ( awl_to_aenv  Γ  )  )  ->
      a_smono_typ  ( awl_to_aenv  Γ  )  B1 ->
      (  forall X1 X2 Γ2 Γ3, X1 `notin` L -> X2 `notin` (L `union` singleton X1) -> 
             (a_update_bound  Γ   nil   X   B1  a_mode_ub__upper  Γ2   Γ3 ) /\  a_wl_red  (   ( awl_app  Γ3   Γ2  )   ) 
      ) ->
      a_wl_red (aworklist_conswork Γ (work_sub (typ_var_f X) B1))
- | a_wlred__sub_intersection1 : forall (Γ:aworklist) (A1 B1 B2:typ),
+ | d_wl_del__sub_intersection1 : forall (Γ:aworklist) (A1 B1 B2:typ),
      a_wl_red (aworklist_conswork (aworklist_conswork Γ (work_sub A1 B1)) (work_sub A1 B2)) ->
      a_wl_red (aworklist_conswork Γ (work_sub A1 (typ_intersection B1 B2)))
- | a_wlred__sub_intersection2 : forall (Γ:aworklist) (B1 B2 A1:typ),
+ | d_wl_del__sub_intersection2 : forall (Γ:aworklist) (B1 B2 A1:typ),
      a_wl_red (aworklist_conswork Γ (work_sub B1 A1)) ->
      a_wl_red (aworklist_conswork Γ (work_sub (typ_intersection B1 B2) A1))
- | a_wlred__sub_intersection3 : forall (Γ:aworklist) (B1 B2 A1:typ),
+ | d_wl_del__sub_intersection3 : forall (Γ:aworklist) (B1 B2 A1:typ),
      a_wl_red (aworklist_conswork Γ (work_sub B2 A1)) ->
      a_wl_red (aworklist_conswork Γ (work_sub (typ_intersection B1 B2) A1))
- | a_wlred__sub_union1 : forall (Γ:aworklist) (B1 A1 A2:typ),
+ | d_wl_del__sub_union1 : forall (Γ:aworklist) (B1 A1 A2:typ),
      a_wl_red (aworklist_conswork Γ (work_sub B1 A1)) ->
      a_wl_red (aworklist_conswork Γ (work_sub B1 (typ_union A1 A2)))
- | a_wlred__sub_union2 : forall (Γ:aworklist) (B1 A1 A2:typ),
+ | d_wl_del__sub_union2 : forall (Γ:aworklist) (B1 A1 A2:typ),
      a_wl_red (aworklist_conswork Γ (work_sub B1 A2)) ->
      a_wl_red (aworklist_conswork Γ (work_sub B1 (typ_union A1 A2)))
- | a_wlred__sub_union3 : forall (Γ:aworklist) (B1 B2 A1:typ),
+ | d_wl_del__sub_union3 : forall (Γ:aworklist) (B1 B2 A1:typ),
      a_wl_red (aworklist_conswork (aworklist_conswork Γ (work_sub B1 A1)) (work_sub B2 A1)) ->
      a_wl_red (aworklist_conswork Γ (work_sub (typ_union B1 B2) A1))
- | a_wlred__chk_sub : forall (Γ:aworklist) (e:exp) (A1:typ),
+ | d_wl_del__chk_sub : forall (Γ:aworklist) (e:exp) (A1:typ),
      a_wl_red (aworklist_conswork Γ (work_infer e (cont_sub A1))) ->
      a_wl_red (aworklist_conswork Γ (work_check e A1))
- | a_wlred__chk_absarrow : forall (L:vars) (Γ:aworklist) (e:exp) (A1 A2:typ),
+ | d_wl_del__chk_absarrow : forall (L:vars) (Γ:aworklist) (e:exp) (A1 A2:typ),
       ( forall x , x \notin  L  -> a_wl_red (aworklist_conswork (aworklist_consvar Γ x (abind_typ A1)) (work_check  ( open_exp_wrt_exp e (exp_var_f x) )  A2)) )  ->
      a_wl_red (aworklist_conswork Γ (work_check (exp_abs e) (typ_arrow A1 A2)))
- | a_wlred__chk_absevar : forall (L:vars) (Γ:aworklist) (e:exp) (X:typvar) (A1 A2:typ) (X1 X2:typvar),
+ | d_wl_del__chk_absevar : forall (L:vars) (Γ:aworklist) (e:exp) (X:typvar) (A1 A2:typ) (X1 X2:typvar),
       binds ( X )  ( (abind_bound A1 A2) ) (  ( awl_to_aenv  Γ  )  )  ->
       (  forall x X1 X2 Γ2 Γ3, x `notin` L -> X1 `notin` (L `union` (singleton x)) -> X2 `notin` (L `union` singleton x `union` singleton X1) -> 
             (a_update_bound  (aworklist_constvar (aworklist_constvar Γ X1 (abind_bound typ_bot typ_top)) X2 (abind_bound typ_bot typ_top))  nil   X   (typ_arrow (typ_var_f X1) (typ_var_f X2))  a_mode_ub__both  Γ2   Γ3 )  /\
             a_wl_red (aworklist_conswork (aworklist_consvar  (   ( awl_app  Γ3   Γ2  )   )  x (abind_typ (typ_var_f X1))) (work_check  ( open_exp_wrt_exp e (exp_var_f x) )  (typ_var_f X2))) ) ->
      a_wl_red (aworklist_conswork Γ (work_check (exp_abs e) (typ_var_f X)))
- | a_wlred__chk_abstop : forall (L:vars) (Γ:aworklist) (e:exp),
+ | d_wl_del__chk_abstop : forall (L:vars) (Γ:aworklist) (e:exp),
       ( forall x , x \notin  L  -> a_wl_red (aworklist_conswork (aworklist_consvar Γ x (abind_typ typ_bot)) (work_check  ( open_exp_wrt_exp e (exp_var_f x) )  typ_top)) )  ->
      a_wl_red (aworklist_conswork Γ (work_check (exp_abs e) typ_top))
- | a_wlred__chk_inter : forall (Γ:aworklist) (e:exp) (A1 A2:typ),
+ | d_wl_del__chk_inter : forall (Γ:aworklist) (e:exp) (A1 A2:typ),
      a_wl_red (aworklist_conswork (aworklist_conswork Γ (work_check e A1)) (work_check e A2)) ->
      a_wl_red (aworklist_conswork Γ (work_check e (typ_intersection A1 A2)))
- | a_wlred__chk_union1 : forall (Γ:aworklist) (e:exp) (A1 A2:typ),
+ | d_wl_del__chk_union1 : forall (Γ:aworklist) (e:exp) (A1 A2:typ),
      a_wl_red (aworklist_conswork Γ (work_check e A1)) ->
      a_wl_red (aworklist_conswork Γ (work_check e (typ_union A1 A2)))
- | a_wlred__chk_union2 : forall (Γ:aworklist) (e:exp) (A1 A2:typ),
+ | d_wl_del__chk_union2 : forall (Γ:aworklist) (e:exp) (A1 A2:typ),
      a_wl_red (aworklist_conswork Γ (work_check e A2)) ->
      a_wl_red (aworklist_conswork Γ (work_check e (typ_union A1 A2)))
- | a_wlred__inf_var : forall (Γ:aworklist) (x:expvar) (c:cont) (A:typ),
+ | d_wl_del__inf_var : forall (Γ:aworklist) (x:expvar) (c:cont) (A:typ),
       binds ( x )  ( (abind_typ A) ) (  ( awl_to_aenv  Γ  )  )  ->
      a_wl_red (aworklist_conswork Γ (work_apply c A)) ->
      a_wl_red (aworklist_conswork Γ (work_infer (exp_var_f x) c))
- | a_wlred__inf_anno : forall (Γ:aworklist) (e:exp) (A:typ) (c:cont),
+ | d_wl_del__inf_anno : forall (Γ:aworklist) (e:exp) (A:typ) (c:cont),
      a_wl_red (aworklist_conswork (aworklist_conswork Γ (work_apply c A)) (work_check e A)) ->
      a_wl_red (aworklist_conswork Γ (work_infer  ( (exp_anno e A) )  c))
- | a_wlred__inf_tabs : forall (L:vars) (Γ:aworklist) (e:exp) (A:typ) (c:cont) (Γ2:aworklist),
+ | d_wl_del__inf_tabs : forall (L:vars) (Γ:aworklist) (e:exp) (A:typ) (c:cont) (Γ2:aworklist),
      lc_aworklist Γ ->
       ( forall X , X \notin  L  -> a_wl_red (aworklist_conswork (aworklist_constvar (aworklist_conswork Γ2 (work_apply c  ( (typ_all A) ) )) X abind_tvar_empty) (work_check  ( open_exp_wrt_typ e (typ_var_f X) )   ( open_typ_wrt_typ A (typ_var_f X) ) )) )  ->
      a_wl_red (aworklist_conswork Γ (work_infer (exp_tabs (body_anno e A)) c))
- | a_wlred__inf_unit : forall (Γ:aworklist) (c:cont),
+ | d_wl_del__inf_unit : forall (Γ:aworklist) (c:cont),
      a_wl_red (aworklist_conswork Γ (work_apply c typ_unit)) ->
      a_wl_red (aworklist_conswork Γ (work_infer exp_unit c))
- | a_wlred__inf_app : forall (Γ:aworklist) (e1 e2:exp) (c:cont),
+ | d_wl_del__inf_app : forall (Γ:aworklist) (e1 e2:exp) (c:cont),
      a_wl_red (aworklist_conswork Γ (work_infer e1  (  (cont_infabs  (  (cont_infapp e2 c)  ) )  ) )) ->
      a_wl_red (aworklist_conswork Γ (work_infer  ( (exp_app e1 e2) )  c))
- | a_wlred__infapp : forall (Γ:aworklist) (A1 A2:typ) (e:exp) (c:cont),
+ | d_wl_del__infapp : forall (Γ:aworklist) (A1 A2:typ) (e:exp) (c:cont),
      a_wl_red (aworklist_conswork (aworklist_conswork Γ (work_apply c A2)) (work_check e A1)) ->
      a_wl_red (aworklist_conswork Γ (work_infapp (typ_arrow A1 A2) e c))
- | a_wlred__infabs_arr : forall (Γ:aworklist) (A1 B1:typ) (c:cont),
+ | d_wl_del__infabs_arr : forall (Γ:aworklist) (A1 B1:typ) (c:cont),
      a_wl_red (aworklist_conswork Γ (work_apply c (typ_arrow A1 B1))) ->
      a_wl_red (aworklist_conswork Γ (work_infabs (typ_arrow A1 B1) c))
- | a_wlred__infabs_bot : forall (Γ:aworklist) (c:cont),
+ | d_wl_del__infabs_bot : forall (Γ:aworklist) (c:cont),
      a_wl_red (aworklist_conswork Γ (work_infabs (typ_arrow typ_top typ_bot) c)) ->
      a_wl_red (aworklist_conswork Γ (work_infabs typ_bot c))
- | a_wlred__infabs_all : forall (L:vars) (Γ:aworklist) (A:typ) (c:cont),
+ | d_wl_del__infabs_all : forall (L:vars) (Γ:aworklist) (A:typ) (c:cont),
      (forall X, X `notin` L -> a_wl_red (aworklist_conswork  (aworklist_constvar Γ X (abind_bound typ_bot typ_top)) (work_infabs (open_typ_wrt_typ A (typ_var_f X)) c)) ) ->
      a_wl_red (aworklist_conswork Γ (work_infabs (typ_all A) c))
- | a_wlred__infabs_inter1 : forall (Γ:aworklist) (A1 A2:typ) (c:cont),
+ | d_wl_del__infabs_inter1 : forall (Γ:aworklist) (A1 A2:typ) (c:cont),
      lc_typ A2 ->
      a_wl_red (aworklist_conswork Γ (work_infabs A1 c)) ->
      a_wl_red (aworklist_conswork Γ (work_infabs (typ_intersection A1 A2) c))
- | a_wlred__infabs_inter2 : forall (Γ:aworklist) (A1 A2:typ) (c:cont),
+ | d_wl_del__infabs_inter2 : forall (Γ:aworklist) (A1 A2:typ) (c:cont),
      lc_typ A1 ->
      a_wl_red (aworklist_conswork Γ (work_infabs A2 c)) ->
      a_wl_red (aworklist_conswork Γ (work_infabs (typ_intersection A1 A2) c))
- | a_wlred__infabs_union : forall (Γ:aworklist) (A1 A2:typ) (c:cont),
+ | d_wl_del__infabs_union : forall (Γ:aworklist) (A1 A2:typ) (c:cont),
      a_wl_red (aworklist_conswork Γ (work_infabs A1  (  (cont_infabsunion A2 c)  ) )) ->
      a_wl_red (aworklist_conswork Γ (work_infabs (typ_union A1 A2) c))
- | a_wlred__infabsunion : forall (Γ:aworklist) (B1 C1 A2:typ) (c:cont),
+ | d_wl_del__infabsunion : forall (Γ:aworklist) (B1 C1 A2:typ) (c:cont),
      a_wl_red (aworklist_conswork Γ (work_infabs A2  (  (cont_unioninfabs (typ_arrow B1 C1) c)  ) )) ->
      a_wl_red (aworklist_conswork Γ (work_infabsunion (typ_arrow B1 C1) A2 c))
- | a_wlred__unioninfabs : forall (Γ:aworklist) (B2 C2 B1 C1:typ) (c:cont),
+ | d_wl_del__unioninfabs : forall (Γ:aworklist) (B2 C2 B1 C1:typ) (c:cont),
      a_wl_red (aworklist_conswork Γ (work_apply c (typ_arrow  ( (typ_intersection B1 B2) )   ( (typ_union C1 C2) ) ))) ->
      a_wl_red (aworklist_conswork Γ (work_unioninfabs (typ_arrow B2 C2) (typ_arrow B1 C1) c))
- | a_wlred__infabs_evar : forall (L:vars) (Γ:aworklist) (X:typvar) (c:cont) (A1 A2:typ) (X1 X2:typvar),
+ | d_wl_del__infabs_evar : forall (L:vars) (Γ:aworklist) (X:typvar) (c:cont) (A1 A2:typ) (X1 X2:typvar),
      binds ( X )  ( (abind_bound A1 A2) ) (  ( awl_to_aenv  Γ  )  )  ->
      (forall X1 X2 Γ2 Γ3, X1 `notin` L -> X2 `notin` (L `union` singleton X1) -> 
        (a_update_bound  (aworklist_constvar (aworklist_constvar Γ X1 (abind_bound typ_bot typ_top)) X2 (abind_bound typ_bot typ_top))   nil   X   (typ_arrow (typ_var_f X1) (typ_var_f X2))  a_mode_ub__both  Γ2   Γ3 )  /\
        a_wl_red (aworklist_conswork  (   ( awl_app  Γ3   Γ2  )   )  (work_infabs (typ_arrow (typ_var_f X1) (typ_var_f X2)) c))
      ) ->
     a_wl_red (aworklist_conswork Γ (work_infabs (typ_var_f X) c))
- | a_wlred__inf_tapp : forall (Γ:aworklist) (e:exp) (B:typ) (c:cont),
+ | d_wl_del__inf_tapp : forall (Γ:aworklist) (e:exp) (B:typ) (c:cont),
      a_wl_red (aworklist_conswork Γ (work_infer e (cont_inftapp B c))) ->
      a_wl_red (aworklist_conswork Γ (work_infer (exp_tapp e B) c))
- | a_wlred__inftapp_all : forall (Γ:aworklist) (A B:typ) (c:cont),
+ | d_wl_del__inftapp_all : forall (Γ:aworklist) (A B:typ) (c:cont),
      a_wl_red (aworklist_conswork Γ (work_apply c  (open_typ_wrt_typ  A   B ) )) ->
      a_wl_red (aworklist_conswork Γ (work_inftapp (typ_all A) B c))
- | a_wlred__inftapp_bot : forall (Γ:aworklist) (B:typ) (c:cont),
+ | d_wl_del__inftapp_bot : forall (Γ:aworklist) (B:typ) (c:cont),
      a_wl_red (aworklist_conswork Γ (work_apply c typ_bot)) ->
      a_wl_red (aworklist_conswork Γ (work_inftapp typ_bot B c))
- | a_wlred__inftapp_inter1 : forall (Γ:aworklist) (A1 A2 B:typ) (c:cont),
+ | d_wl_del__inftapp_inter1 : forall (Γ:aworklist) (A1 A2 B:typ) (c:cont),
      a_wl_red (aworklist_conswork Γ (work_inftapp A1 B c)) ->
      a_wl_red (aworklist_conswork Γ (work_inftapp (typ_intersection A1 A2) B c))
- | a_wlred__inftapp_inter2 : forall (Γ:aworklist) (A1 A2 B:typ) (c:cont),
+ | d_wl_del__inftapp_inter2 : forall (Γ:aworklist) (A1 A2 B:typ) (c:cont),
      a_wl_red (aworklist_conswork Γ (work_inftapp A2 B c)) ->
      a_wl_red (aworklist_conswork Γ (work_inftapp (typ_intersection A1 A2) B c))
- | a_wlred__inftapp_union : forall (Γ:aworklist) (A1 A2 B:typ) (c:cont),
+ | d_wl_del__inftapp_union : forall (Γ:aworklist) (A1 A2 B:typ) (c:cont),
      a_wl_red (aworklist_conswork Γ (work_inftapp A1 B  (  (cont_inftappunion A2 B c)  ) )) ->
      a_wl_red (aworklist_conswork Γ (work_inftapp (typ_union A1 A2) B c))
- | a_wlred__inftappunion : forall (Γ:aworklist) (C1 A2 B:typ) (c:cont),
+ | d_wl_del__inftappunion : forall (Γ:aworklist) (C1 A2 B:typ) (c:cont),
      a_wl_red (aworklist_conswork Γ (work_inftapp A2 B  (  (cont_unioninftapp C1 c)  ) )) ->
      a_wl_red (aworklist_conswork Γ (work_inftappunion C1 A2 B c))
- | a_wlred__unioninftapp : forall (Γ:aworklist) (C2 C1:typ) (c:cont),
+ | d_wl_del__unioninftapp : forall (Γ:aworklist) (C2 C1:typ) (c:cont),
      a_wl_red (aworklist_conswork Γ (work_apply c (typ_union C1 C2))) ->
      a_wl_red (aworklist_conswork Γ (work_unioninftapp C2 C1 c))
  | d_wl_red__applycont : forall (Γ:aworklist) (w:work) (T1:typ) (c:cont),
